structure

Cslib/Computability/LambdaCalculus/STLC/LocallyNameless/Basic.lean
@@ -4,9 +4,7 @@ Released under Apache 2.0 license as described in the file LICENSE.
 Authors: Chris Henson
 -/
 
-import Cslib.Computability.LambdaCalculus.Untyped.LocallyNameless.Basic
-import Cslib.Computability.LambdaCalculus.Untyped.LocallyNameless.Properties
-import Cslib.Computability.LambdaCalculus.Untyped.LocallyNameless.FullBetaConfluence
+import Cslib.Computability.LambdaCalculus.STLC.LocallyNameless.Context
 
 /-! # λ-calculus
 
@@ -36,187 +34,13 @@ inductive Ty
 scoped infixr:70 " ⤳ " => Ty.arrow
 scoped prefix:90 "~ " => Ty.base
 
-/-- A typing context is a list of free variables and corresponding types. -/
-abbrev Ctx (Var : Type u) := List (Var × Ty)
-
-/-- The domain of a context is the finite set of free variables it uses. -/
-@[simp]
-def Ctx.dom : Ctx Var → Finset Var := λ Γ ↦ Γ.map Prod.fst |>.toFinset
-
-/-- A well-formed context. -/
-inductive Ok : Ctx Var → Prop
-| nil : Ok []
-| cons : Ok Γ → x ∉ Γ.dom → Ok ((x,σ) :: Γ)
-
-/-- Context membership is preserved on permuting a context. -/
-theorem Ctx.dom_perm_mem_iff {Γ Δ : Ctx Var} (h : Γ.Perm Δ) {x : Var} : 
-    x ∈ Γ.dom ↔ x ∈ Δ.dom := by
-  induction h <;> aesop
-
-theorem Ctx.dom_perm_nmem {Γ Δ : Ctx Var} (h : Γ.Perm Δ) {x : Var} : 
-    x ∉ Γ.dom → x ∉ Δ.dom := by
-  intros Γ_nmem Δ_mem
-  apply Γ_nmem
-  exact (dom_perm_mem_iff h).mpr Δ_mem
-
-/-- Context well-formedness is preserved on permuting a context. -/
-@[aesop safe forward (rule_sets := [LambdaCalculus.LocallyNameless.ruleSet])]
-theorem Ok.perm {Γ Δ : Ctx Var} (h : Γ.Perm Δ) : Ok Γ → Ok Δ := by
-  induction h <;> intro Γ_ok
-  case cons perm ih =>
-    cases Γ_ok
-    case cons ok_Γ mem => exact Ok.cons (ih ok_Γ) (Ctx.dom_perm_nmem perm mem)
-  case nil => constructor
-  case trans => simp_all
-  case swap =>
-    cases Γ_ok
-    case cons ok _ =>
-    cases ok
-    case cons ok _ =>
-      constructor
-      constructor
-      all_goals aesop
-
 open Term Ty
 
 /-- An extrinsic typing derivation for locally nameless terms. -/
 @[aesop unsafe [constructors (rule_sets := [LambdaCalculus.LocallyNameless.ruleSet])]]
-inductive Typing : Ctx Var → Term Var → Ty → Prop
-| var : Ok Γ → (x,σ) ∈ Γ → Typing Γ (fvar x) σ
+inductive Typing : Ctx Var Ty → Term Var → Ty → Prop
+| var : Γ.Ok → (x,σ) ∈ Γ → Typing Γ (fvar x) σ
 | abs (L : Finset Var) : (∀ x ∉ L, Typing ((x,σ) :: Γ) (t ^ fvar x) τ) → Typing Γ t.abs (σ ⤳ τ) 
 | app : Typing Γ t (σ ⤳ τ) → Typing Γ t' σ → Typing Γ (app t t') τ
 
 scoped notation:50 Γ " ⊢ " t " ∶" τ:arg => Typing Γ t τ
-
-variable {Γ Δ Φ : Ctx Var}
-
-/-- Typing is preserved on permuting a context. -/
-theorem Typing.perm : Γ.Perm Δ → Γ ⊢ t ∶ τ → Δ ⊢ t ∶ τ := by 
-  intros _ der
-  revert Δ
-  induction der <;> intros Δ p
-  case app => aesop
-  case var => 
-    have := @p.mem_iff
-    aesop
-  case abs ih => 
-    constructor
-    intros x mem
-    exact ih x mem (by aesop)
-
-open List Finset in
-private lemma weakening_strengthened_eq (eq : Γ_Δ  = Γ ++ Δ) : 
-    Γ_Δ  ⊢ t ∶ τ → Ok (Γ ++ Φ ++ Δ) → (Γ ++ Φ ++ Δ) ⊢ t ∶ τ := by
-  intros h
-  revert Γ Δ Φ
-  induction h <;> intros Γ Δ Φ eq ok_Γ_Φ_Δ
-  case var => aesop
-  case app => aesop
-  case abs σ Γ' τ t xs ext ih =>
-    apply Typing.abs (xs ∪ (Γ ++ Φ ++ Δ).dom)
-    intros x _
-    have h : (x, σ) :: Γ' = (x, σ) :: Γ ++ Δ := by aesop
-    refine @ih x (by aesop) _ _ Φ h ?_
-    constructor <;> aesop
-
-/-- Weakening of a typing derivation with an appended context. -/
-lemma weakening_strengthened : 
-    Γ ++ Δ ⊢ t ∶ τ → Ok (Γ ++ Φ ++ Δ) → (Γ ++ Φ ++ Δ) ⊢ t ∶ τ :=
-  weakening_strengthened_eq rfl
-
-/-- Weakening of a typing derivation by an additional context. -/
-lemma weakening : Γ ⊢ t ∶ T → Ok (Γ ++ Δ) → Γ ++ Δ ⊢ t ∶ T := by
-  intros der ok
-  rw [←List.append_nil (Γ ++ Δ)] at *
-  exact weakening_strengthened (by simp_all) ok
-
-/-- Typing derivations exist only for locally closed terms. -/
-lemma typing_lc : Γ ⊢ t ∶ τ → t.LC := by
-  intros h
-  induction h <;> constructor
-  case abs ih => exact ih
-  all_goals aesop
-
-variable [HasFresh Var]
-
-private lemma typing_subst_strengthened_eq (eq : Φ = Δ ++ (x, σ) :: Γ) :
-    Φ ⊢ t ∶ τ →
-    Γ ⊢ s ∶ σ → 
-    (Δ ++ Γ) ⊢ (t [x := s]) ∶ τ := by
-  intros h
-  revert Γ Δ
-  induction h <;> intros Γ Δ eq der
-  case app => aesop
-  case var x' τ ok mem => 
-    simp only [subst_fvar]
-    rw [eq] at mem
-    rw [eq] at ok
-    cases (Ok.perm (by aesop) ok : Ok ((x, σ) :: Δ ++ Γ))
-    case cons ok_weak _ =>
-    observe perm : (Γ ++ Δ).Perm (Δ ++ Γ)
-    by_cases h : x = x' <;> simp only [h]
-    · rw [show τ = σ by aesop]
-      refine Typing.perm perm (weakening der ?_)
-      exact Ok.perm (id (List.Perm.symm perm)) ok_weak
-    · aesop
-  case abs σ Γ' t T2 xs ih' ih =>
-    apply Typing.abs (xs ∪ {x} ∪ (Δ ++ Γ).dom)
-    intros x _
-    rw [
-      subst_def, 
-      subst_open_var _ _ _ _ _ (typing_lc der),
-      show (x, σ) :: (Δ ++ Γ) = ((x, σ) :: Δ) ++ Γ by aesop
-      ]
-    apply ih 
-    all_goals aesop  
-
-/-- Substitution for a context weakened by a single type between appended contexts. -/
-lemma typing_subst_strengthened :
-  (Δ ++ (z, S) :: Γ) ⊢ t ∶ T →
-  Γ ⊢ s ∶ S → 
-  (Δ ++ Γ) ⊢ (t [z := s]) ∶ T
-  := typing_subst_strengthened_eq rfl
-
-/-- Substitution for a context weakened by a single type. -/
-lemma typing_subst : 
-    (x, σ) :: Γ ⊢ t ∶ τ  → Γ ⊢ s ∶ σ → Γ ⊢ (t [x := s]) ∶ τ := by
-  intros weak der
-  rw [←List.nil_append Γ]
-  exact typing_subst_strengthened weak der
-
-/-- Typing preservation for opening. -/
-@[aesop safe forward (rule_sets := [LambdaCalculus.LocallyNameless.ruleSet])]
-theorem preservation_opening {xs : Finset Var} :
-  (∀ x ∉ xs, (x, σ) :: Γ ⊢ m ^ fvar x ∶ τ) → 
-  Γ ⊢ n ∶ σ → Γ ⊢ m ^ n ∶ τ
-  := by
-  intros mem der
-  have ⟨fresh, free⟩ := fresh_exists (xs ∪ m.fv)
-  rw [subst_intro fresh n m (by aesop) (typing_lc der)]
-  refine typing_subst (mem fresh (by aesop)) der
-
-/-- Typing preservation. -/
-@[aesop safe forward (rule_sets := [LambdaCalculus.LocallyNameless.ruleSet])]
-theorem preservation : Γ ⊢ t ∶ τ → (t ⭢βᶠt') → Γ ⊢ t' ∶ τ := by
-  intros der
-  revert t'
-  induction der <;> intros t' step <;> cases step
-  case' abs.abs xs _ _ _ xs' _=> apply Typing.abs (xs ∪ xs')
-  case' app.beta der_l _ _ => cases der_l
-  all_goals aesop
-
-/-- Typing preservation for multiple steps of reduction. -/
-theorem preservation_redex : Γ ⊢ t ∶ T → (t ↠βᶠ t') → Γ ⊢ t' ∶ T := by
-  intros der redex
-  induction redex using Relation.ReflTransGen.trans_induction_on <;> aesop
-
-/-- Typing preservation for confluence. -/
-theorem preservation_confluence :
-    Γ ⊢ a ∶ τ → (a ↠βᶠ b) → (a ↠βᶠ c) → 
-    ∃ d, (b ↠βᶠ d) ∧ (c ↠βᶠ d) ∧ Γ ⊢ d ∶ τ := by
-  intros der ab ac
-  have ⟨d, bd, cd⟩ := confluence_beta ab ac
-  refine ⟨d, bd, cd, preservation_redex der ?_⟩
-  trans
-  exact ab
-  exact bd
