Cslib/Computability/LambdaCalculus/STLC/LocallyNameless/Context.lean
@@ -1,0 +1,65 @@
+/-
+Copyright (c) 2025 Chris Henson. All rights reserved.
+Released under Apache 2.0 license as described in the file LICENSE.
+Authors: Chris Henson
+-/
+
+import Cslib.Computability.LambdaCalculus.Untyped.LocallyNameless.Basic
+
+/-! # λ-calculus
+
+Contexts as pairs of free variables and types.
+
+-/
+
+universe u v
+
+variable {Var : Type u} {Ty : Type v} [DecidableEq Var]
+
+namespace LambdaCalculus.LocallyNameless
+
+/-- A typing context is a list of free variables and corresponding types. -/
+abbrev Ctx (Var : Type u) (Ty : Type v) := List (Var × Ty)
+
+namespace Ctx
+
+/-- The domain of a context is the finite set of free variables it uses. -/
+@[simp]
+def dom : Ctx Var Ty → Finset Var := λ Γ ↦ Γ.map Prod.fst |>.toFinset
+
+/-- A well-formed context. -/
+inductive Ok : Ctx Var Ty → Prop
+| nil : Ok []
+| cons : Ok Γ → x ∉ Γ.dom → Ok ((x,σ) :: Γ)
+
+variable {Γ Δ : Ctx Var Ty}
+
+/-- Context membership is preserved on permuting a context. -/
+theorem dom_perm_mem_iff (h : Γ.Perm Δ) {x : Var} : 
+    x ∈ Γ.dom ↔ x ∈ Δ.dom := by
+  induction h <;> aesop
+
+/-- Context non-membership is preserved on permuting a context. -/
+theorem dom_perm_nmem (h : Γ.Perm Δ) {x : Var} : 
+    x ∉ Γ.dom → x ∉ Δ.dom := by
+  intros Γ_nmem Δ_mem
+  apply Γ_nmem
+  exact (dom_perm_mem_iff h).mpr Δ_mem
+
+/-- Context well-formedness is preserved on permuting a context. -/
+@[aesop safe forward (rule_sets := [LambdaCalculus.LocallyNameless.ruleSet])]
+theorem perm (h : Γ.Perm Δ) : Ok Γ → Ok Δ := by
+  induction h <;> intro Γ_ok
+  case cons perm ih =>
+    cases Γ_ok
+    case cons ok_Γ mem => exact Ok.cons (ih ok_Γ) (Ctx.dom_perm_nmem perm mem)
+  case nil => constructor
+  case trans => simp_all
+  case swap =>
+    cases Γ_ok
+    case cons ok _ =>
+    cases ok
+    case cons ok _ =>
+      constructor
+      constructor
+      all_goals aesop
