Cslib/Computability/LambdaCalculus/STLC/LocallyNameless/Safety.lean
@@ -1,0 +1,176 @@
+/-
+Copyright (c) 2025 Chris Henson. All rights reserved.
+Released under Apache 2.0 license as described in the file LICENSE.
+Authors: Chris Henson
+-/
+
+import Cslib.Computability.LambdaCalculus.STLC.LocallyNameless.Basic
+import Cslib.Computability.LambdaCalculus.Untyped.LocallyNameless.Basic
+import Cslib.Computability.LambdaCalculus.Untyped.LocallyNameless.Properties
+import Cslib.Computability.LambdaCalculus.Untyped.LocallyNameless.FullBetaConfluence
+
+/-! # λ-calculus
+
+Typing preservation of the simply typed λ-calculus, with a locally nameless representation of syntax.
+
+## References
+
+* [A. Chargueraud, *The Locally Nameless Representation*] [Chargueraud2012]
+* See also https://www.cis.upenn.edu/~plclub/popl08-tutorial/code/, from which
+  this is partially adapted
+
+-/
+
+universe u
+
+variable {Var : Type u} [DecidableEq Var]
+
+namespace LambdaCalculus.LocallyNameless.Typing
+
+variable {Γ Δ Φ : Ctx Var Ty}
+
+/-- Typing is preserved on permuting a context. -/
+theorem perm : Γ.Perm Δ → Γ ⊢ t ∶ τ → Δ ⊢ t ∶ τ := by 
+  intros _ der
+  revert Δ
+  induction der <;> intros Δ p
+  case app => aesop
+  case var => 
+    have := @p.mem_iff
+    aesop
+  case abs ih => 
+    constructor
+    intros x mem
+    exact ih x mem (by aesop)
+
+open List Finset in
+private lemma weakening_strengthened_eq (eq : Γ_Δ  = Γ ++ Δ) : 
+    Γ_Δ  ⊢ t ∶ τ → (Γ ++ Φ ++ Δ).Ok → (Γ ++ Φ ++ Δ) ⊢ t ∶ τ := by
+  intros h
+  revert Γ Δ Φ
+  induction h <;> intros Γ Δ Φ eq ok_Γ_Φ_Δ
+  case var => aesop
+  case app => aesop
+  case abs σ Γ' τ t xs ext ih =>
+    apply Typing.abs (xs ∪ (Γ ++ Φ ++ Δ).dom)
+    intros x _
+    have h : (x, σ) :: Γ' = (x, σ) :: Γ ++ Δ := by aesop
+    refine @ih x (by aesop) _ _ Φ h ?_
+    constructor <;> aesop
+
+/-- Weakening of a typing derivation with an appended context. -/
+lemma weakening_strengthened : 
+    Γ ++ Δ ⊢ t ∶ τ → (Γ ++ Φ ++ Δ).Ok → (Γ ++ Φ ++ Δ) ⊢ t ∶ τ :=
+  weakening_strengthened_eq rfl
+
+/-- Weakening of a typing derivation by an additional context. -/
+lemma weakening : Γ ⊢ t ∶ T → (Γ ++ Δ).Ok → Γ ++ Δ ⊢ t ∶ T := by
+  intros der ok
+  rw [←List.append_nil (Γ ++ Δ)] at *
+  exact weakening_strengthened (by simp_all) ok
+
+/-- Typing derivations exist only for locally closed terms. -/
+lemma lc : Γ ⊢ t ∶ τ → t.LC := by
+  intros h
+  induction h <;> constructor
+  case abs ih => exact ih
+  all_goals aesop
+
+variable [HasFresh Var]
+
+open Term
+
+private lemma subst_strengthened_eq (eq : Φ = Δ ++ (x, σ) :: Γ) :
+    Φ ⊢ t ∶ τ →
+    Γ ⊢ s ∶ σ → 
+    (Δ ++ Γ) ⊢ (t [x := s]) ∶ τ := by
+  intros h
+  revert Γ Δ
+  induction h <;> intros Γ Δ eq der
+  case app => aesop
+  case var x' τ ok mem => 
+    simp only [subst_fvar]
+    rw [eq] at mem
+    rw [eq] at ok
+    cases (Ctx.perm (by aesop) ok : @Ctx.Ok Var Ty _ ((x, σ) :: Δ ++ Γ))
+    case cons ok_weak _ =>
+    observe perm : (Γ ++ Δ).Perm (Δ ++ Γ)
+    by_cases h : x = x' <;> simp only [h]
+    · rw [show τ = σ by aesop]
+      refine Typing.perm perm (weakening der ?_)
+      exact Ctx.perm (id (List.Perm.symm perm)) ok_weak
+    · aesop
+  case abs σ Γ' t T2 xs ih' ih =>
+    apply Typing.abs (xs ∪ {x} ∪ (Δ ++ Γ).dom)
+    intros x _
+    rw [
+      subst_def, 
+      subst_open_var _ _ _ _ _ der.lc,
+      show (x, σ) :: (Δ ++ Γ) = ((x, σ) :: Δ) ++ Γ by aesop
+      ]
+    apply ih 
+    all_goals aesop  
+
+/-- Substitution for a context weakened by a single type between appended contexts. -/
+lemma subst_strengthened :
+  (Δ ++ (x, σ) :: Γ) ⊢ t ∶ τ →
+  Γ ⊢ s ∶ σ → 
+  (Δ ++ Γ) ⊢ (t [x := s]) ∶ τ := subst_strengthened_eq rfl
+
+/-- Substitution for a context weakened by a single type. -/
+lemma typing_subst : 
+    (x, σ) :: Γ ⊢ t ∶ τ  → Γ ⊢ s ∶ σ → Γ ⊢ (t [x := s]) ∶ τ := by
+  intros weak der
+  rw [←List.nil_append Γ]
+  exact subst_strengthened weak der
+
+/-- Typing preservation for opening. -/
+@[aesop safe forward (rule_sets := [LambdaCalculus.LocallyNameless.ruleSet])]
+theorem preservation_opening {xs : Finset Var} :
+  (∀ x ∉ xs, (x, σ) :: Γ ⊢ m ^ fvar x ∶ τ) → 
+  Γ ⊢ n ∶ σ → Γ ⊢ m ^ n ∶ τ
+  := by
+  intros mem der
+  have ⟨fresh, free⟩ := fresh_exists (xs ∪ m.fv)
+  rw [subst_intro fresh n m (by aesop) der.lc]
+  refine typing_subst (mem fresh (by aesop)) der
+
+/-- Typing preservation. -/
+@[aesop safe forward (rule_sets := [LambdaCalculus.LocallyNameless.ruleSet])]
+theorem preservation : Γ ⊢ t ∶ τ → (t ⭢βᶠt') → Γ ⊢ t' ∶ τ := by
+  intros der
+  revert t'
+  induction der <;> intros t' step <;> cases step
+  case' abs.abs xs _ _ _ xs' _=> apply Typing.abs (xs ∪ xs')
+  case' app.beta der_l _ _ => cases der_l
+  all_goals aesop
+
+/-- Typing preservation for multiple steps of reduction. -/
+theorem preservation_redex : Γ ⊢ t ∶ T → (t ↠βᶠ t') → Γ ⊢ t' ∶ T := by
+  intros der redex
+  induction redex using Relation.ReflTransGen.trans_induction_on <;> aesop
+
+/-- Typing preservation for confluence. -/
+theorem preservation_confluence :
+    Γ ⊢ a ∶ τ → (a ↠βᶠ b) → (a ↠βᶠ c) → 
+    ∃ d, (b ↠βᶠ d) ∧ (c ↠βᶠ d) ∧ Γ ⊢ d ∶ τ := by
+  intros der ab ac
+  have ⟨d, bd, cd⟩ := confluence_beta ab ac
+  refine ⟨d, bd, cd, preservation_redex der ?_⟩
+  trans
+  exact ab
+  exact bd
+
+/-- A typed term either reduces or is a value. -/
+theorem progress : ([] : Ctx Var Ty) ⊢ t ∶ τ → t.Value ∨ ∃ t', t ⭢βᶠ t' := by
+  intros der
+  generalize eq : [] = Γ at der
+  induction der
+  case var => aesop
+  case abs xs mem ih =>
+    left
+    constructor
+    apply Term.LC.abs xs
+    intros _ mem'
+    exact (mem _ mem').lc
+  case app t _ _ t' der_l der_r ih_l ih_r => sorry
